Prove the sync/smart_sync semaphore

formal-proofs/theories/lib/interruptible_semaphore/interruptible_semaphore.v
@@ -12,33 +12,38 @@ Definition newSemaphore: val :=
   λ: "n", (ref "n", newThreadQueue array_interface #()).
 
 Definition acquireSemaphore: val :=
-  λ: "sem",
-  let: "availablePermits" := Fst ("sem") in
-  let: "e" := Fst (Snd ("sem")) in
-  let: "p" := FAA "availablePermits" #(-1) in
-  if: #0 < "p" then fillThreadQueueFuture #()
-  else suspend array_interface "e".
+  rec: "loop" "sem" :=
+    let: "availablePermits" := Fst ("sem") in
+    let: "e" := Fst (Snd ("sem")) in
+    let: "p" := FAA "availablePermits" #(-1) in
+    if: #0 < "p" then fillThreadQueueFuture #()
+    else match: suspend array_interface "e" with
+             NONE => "loop" "sem"
+           | SOME "v" => "v"
+         end.
 
 Definition semaphoreResume: val :=
   λ: "d", resume array_interface #(Z.of_nat 300) #true #true #false "d"
                  (λ: <>, #()) #().
 
 Definition releaseSemaphore: val :=
-  λ: "sem",
-  let: "availablePermits" := Fst ("sem") in
-  let: "d" := Snd (Snd ("sem")) in
-  let: "p" := FAA "availablePermits" #1 in
-  if: #0 ≤ "p" then #()
-  else semaphoreResume "d".
+  rec: "loop" "sem" :=
+    let: "availablePermits" := Fst ("sem") in
+    let: "d" := Snd (Snd ("sem")) in
+    let: "p" := FAA "availablePermits" #1 in
+    if: #0 ≤ "p" then #()
+    else if: semaphoreResume "d"
+         then #()
+         else "loop" "sem".
 
 Definition cancelSemaphoreFuture : val :=
   λ: "sem" "f",
   let: "availablePermits" := Fst ("sem") in
   let: "d" := Snd (Snd ("sem")) in
   tryCancelThreadQueueFuture' array_interface
-                              #false #(Z.of_nat 300) #true #true #false
+                              #false #(Z.of_nat 300) #true #true
                               "d" (λ: <>, FAA "availablePermits" #1 < #0)
-                              (λ: <>, #()) (λ: <>, releaseSemaphore "sem").
+                              (λ: <>, #()) (λ: <>, releaseSemaphore "sem") "f".
 
 End impl.
 
@@ -73,6 +78,9 @@ Let tqParams R :=
 
 Let isThreadQueue R := is_thread_queue NTq NFuture (tqParams R) _ array_spec.
 
+Definition is_semaphore_future R :=
+  is_thread_queue_future NTq NFuture (tqParams R) _ array_spec.
+
 Definition is_semaphore R γa γtq γe γd (s: val): iProp :=
   ∃ e d (p: loc), ⌜s = (#p, (e, d))%V⌝ ∧
   inv NSem (∃ availablePermits, semaphore_inv R γtq availablePermits p)
@@ -92,9 +100,9 @@ Proof.
   iApply "HΦ". iExists _, _, _. iSplitR; first done. by iFrame "HInv HTq".
 Qed.
 
-Lemma resumeSemaphore_spec R maxWait γa γtq γe γd e d:
+Lemma resumeSemaphore_spec R maxWait (wait: bool) γa γtq γe γd e d:
   {{{ isThreadQueue R γa γtq γe γd e d ∗ awakening_permit γtq }}}
-    resume array_interface #(Z.of_nat maxWait) #true #true #false d (λ: <>, #())%V #()
+    resume array_interface #(Z.of_nat maxWait) #true #true #wait d (λ: <>, #())%V #()
   {{{ (r: bool), RET #r; if r then True else R }}}.
 Proof.
   iIntros (Φ) "[#HTq HAwak] HΦ".
@@ -111,7 +119,7 @@ Theorem releaseSemaphore_spec R γa γtq γe γd s:
     releaseSemaphore array_interface s
   {{{ RET #(); True }}}.
 Proof.
-  iIntros (Φ) "[#HIsSem HR] HΦ". wp_lam.
+  iIntros (Φ) "[#HIsSem HR] HΦ". wp_lam. iLöb as "IH".
   iDestruct "HIsSem" as (e d p ->) "[HInv HTq]". wp_pures. wp_bind (FAA _ _).
   iInv "HInv" as (availablePermits) "[HRs HOpen]" "HClose".
   iDestruct "HOpen" as (enqueuedThreads) "(HState & Hp & >HPures)".
@@ -134,256 +142,128 @@ Proof.
       by replace (availablePermits - enqueuedThreads + 1)%Z with
           (availablePermits - (enqueuedThreads - 1)%nat)%Z by lia. }
     iModIntro. wp_pures. rewrite bool_decide_false; last lia. wp_pures.
-    wp_lam. wp_pures. iApply (resumeSemaphore_spec with "[$]").
-    iIntros "!>" (r) "Hr".
-Abort.
+    wp_lam. wp_pures. wp_apply (resumeSemaphore_spec with "[$]").
+    iIntros (r) "Hr".
+    destruct r; wp_pures. by iApply "HΦ".
+    wp_lam. iApply ("IH" with "Hr HΦ").
+Qed.
 
-Theorem acquire_semaphore_spec Nint R γ (p epℓ eℓ dpℓ dℓ: loc) γa γtq γe γd
-        γi cancHandle γth (threadHandle: loc):
-  is_interrupt_handle Nint γi cancHandle -∗
-  is_thread_handle Nth γth #threadHandle -∗
-  is_semaphore R γ p epℓ eℓ dpℓ dℓ γa γtq γe γd -∗
-  inv (N .@ "permits") (∃ a, semaphore_permits γ a) -∗
-  {{{ thread_doesnt_have_permits γth }}}
-    (acquire_semaphore segment_size) cancHandle #threadHandle #p #epℓ #eℓ #dpℓ #dℓ
-  {{{ (v: val), RET v;
-      ⌜v = InjRV #()⌝ ∧ thread_doesnt_have_permits γth ∗ R ∨
-      ⌜v = InjLV #()⌝ ∧ interrupted γi
-  }}}.
+Theorem acquireSemaphore_spec R γa γtq γe γd s:
+  {{{ is_semaphore R γa γtq γe γd s }}}
+    acquireSemaphore array_interface s
+  {{{ γf v, RET v; is_semaphore_future R γtq γa γf v ∗
+                   thread_queue_future_cancellation_permit γf }}}.
 Proof.
-  iIntros "#HIntHandle #HThreadHandle #HSemInv #HPermInv".
-  iIntros (Φ) "!> HNoPerms HΦ".
-
-  wp_lam. wp_pures. wp_bind (FAA _ _).
-  iInv "HSemInv" as (availablePermits v)
-                      "(HPerms & >HAuth & HTq & Hp & >HPure)" "HInvClose".
-  wp_faa.
-  iInv "HPermInv" as (?) ">HFrag" "HPermsClose".
-  iDestruct (own_valid_2 with "HAuth HFrag") as
-        %[->%Excl_included%leibniz_equiv _]%auth_both_valid.
-  remember (availablePermits - _)%Z as oldP.
-  destruct (decide (0 < oldP)%Z).
-  {
-    iMod (own_update_2 with "HAuth HFrag") as "[HAuth HFrag]".
-    {
-      apply auth_update, option_local_update.
-      apply (exclusive_local_update _ (Excl (availablePermits - 1)%nat)).
-      done.
+  iIntros (Φ) "#HIsSem HΦ". wp_lam. iLöb as "IH".
+  iDestruct "HIsSem" as (e d p ->) "[HInv HTq]". wp_pures. wp_bind (FAA _ _).
+  iInv "HInv" as (availablePermits) "[HRs HOpen]" "HClose".
+  iDestruct "HOpen" as (enqueuedThreads) "(HState & Hp & >HPures)".
+  iDestruct "HPures" as %HPures.
+  destruct (decide (0 < availablePermits - enqueuedThreads)%Z) as [HGe|HLt].
+  - assert (enqueuedThreads = 0) as -> by lia. rewrite Z.sub_0_r.
+    destruct availablePermits as [|availablePermits']=> /=; first lia.
+    iDestruct "HRs" as "[HR HRs]".
+    wp_faa. iMod ("HClose" with "[-HΦ HR]") as "_".
+    { iExists availablePermits'. iFrame "HRs". iExists 0.
+      iFrame "HState". iSplitL; last by iPureIntro; lia.
+      replace (S availablePermits' + -1)%Z with (Z.of_nat availablePermits')
+        by lia.
+      by rewrite Z.sub_0_r. }
+    iModIntro. wp_pures. iApply (fillThreadQueueFuture_spec with "[HR]").
+    2: {
+      iIntros "!>" (γf v') "[HFuture HCancPermit]".
+      iApply "HΦ". iFrame.
     }
-    iMod ("HPermsClose" with "[HFrag]") as "_"; first by eauto.
-    iDestruct "HPure" as %[->|HH].
-    by lia.
-    destruct availablePermits; simpl in *; first by lia.
-    iDestruct "HPerms" as "[HR HPerms]".
-    iSpecialize ("HΦ" with "[HNoPerms HR]").
-    { iLeft. iFrame. eauto. }
-    iMod ("HInvClose" with "[-HΦ]") as "_".
-    {
-      iExists _, _.
-      rewrite Nat.sub_0_r big_opL_irrelevant_element' seq_length.
-      replace (oldP + -1)%Z with (availablePermits - v)%Z by lia.
-      iFrame.
-      iPureIntro.
-      eauto.
-    }
-    iModIntro. wp_pures. rewrite bool_decide_decide decide_True //. by wp_pures.
-  }
+    rewrite /V'. iExists _. iSplitR; first done. simpl.
+    iSplitR; first done. iFrame.
+  - iMod (thread_queue_append' with "HTq [] HState")
+      as "[HState HSus]"=> /=; [by solve_ndisj|done|].
+    wp_faa. iMod ("HClose" with "[-HΦ HSus]") as "_".
+    { iExists availablePermits. iFrame "HRs". iExists (S enqueuedThreads).
+      iFrame "HState". iSplitL; last by iPureIntro; lia.
+      by replace (availablePermits - enqueuedThreads + -1)%Z with
+          (availablePermits - S enqueuedThreads)%Z by lia. }
+    iModIntro. wp_pures. rewrite bool_decide_false; last lia. wp_pures.
+    wp_apply (suspend_spec with "[$]")=> /=. iIntros (v) "[[-> _]|Hv]".
+    + wp_pures. wp_lam. iApply ("IH" with "HΦ").
+    + iDestruct "Hv" as (γf v') "(-> & HFuture & HCancPermit)". wp_pures.
+      iApply "HΦ". iFrame.
+Qed.
 
-  destruct availablePermits.
-  2: by iDestruct "HPure" as %[HContra|HOk]; lia.
-  rewrite Z.sub_0_l in HeqoldP.
-  subst.
-  iClear "HPure".
-  iMod (thread_queue_as_counter_append with "[$] HTq") as "[HIsSusp HTq]".
-  iMod ("HPermsClose" with "[HFrag]") as "_"; first by eauto.
-  iMod ("HInvClose" with "[-HIsSusp HNoPerms HΦ]") as "_".
-  {
-    iExists _, _. iFrame. replace (0%nat - S v)%Z with (-v + - 1)%Z by lia.
-    iFrame.
-    iPureIntro. lia.
-  }
-  iModIntro. wp_pures. rewrite bool_decide_decide decide_False //. wp_pures.
-  wp_lam. wp_pures. wp_lam. wp_pures.
-
-  rewrite /is_semaphore.
-
-  awp_apply (try_enque_thread_as_counter_spec (N.@"tq") with
-                 "HThreadHandle HIsSusp HNoPerms") without "HΦ".
-  iInv "HSemInv" as (? v') "(HPerms & >HAuth & HTq & Hp & >HPure)".
-  iAaccIntro with "HTq".
-  {
-    iIntros "HTq !>". iSplitL; last done.
-    iExists _, _. iFrame.
-  }
-  iIntros (?) "[HTq HPures]".
-  iDestruct "HPures" as "[HPures|(-> & HR & HNoPerms)]".
-  2: {
-    iModIntro. iSplitR "HNoPerms HR".
-    by iExists _, _; iFrame.
-    iIntros "HΦ".
-    wp_pures.
-    iSpecialize ("HΦ" with "[-]").
-    { iLeft. iFrame. eauto. }
-    done.
-  }
-  iDestruct "HPures" as (i s ->) "(#HSegLoc & #HRend & HInhToken)".
-  iSplitR "HInhToken"; first by iExists _, _; iFrame.
-
-  iIntros "!> HΦ". wp_pures. wp_lam. wp_pures.
-  wp_apply (interruptibly_spec _ (inhabitant_token γtq i)
-                               (fun v => ⌜v = #()⌝ ∧ thread_doesnt_have_permits γth ∗ R)%I
-                               (fun v => ⌜v = #()⌝ ∧ interrupted γi)%I
-              with "[HInhToken]").
-  {
-
-    iFrame "HIntHandle HInhToken".
-    iSplit.
-    {
-      iIntros (Φ') "!> HInhTok HΦ'". wp_pures. wp_bind (!_)%E.
-      rewrite /is_thread_handle.
-      awp_apply (thread_queue_as_counter_check_thread_permits_spec with
-                     "HThreadHandle HSegLoc HRend") without "HΦ'".
-      iInv "HSemInv" as (? ?) "(HPerms & >HAuth & HTq & HRest)".
-      iCombine "HInhTok" "HTq" as "HAacc".
-      iAaccIntro with "HAacc".
-      { iIntros "[$ HTq]". by iExists _, _; iFrame. }
-      iIntros (b) "[HTq HRes] !>".
-      iSplitR "HRes".
-      by iExists _, _; iFrame.
-      iIntros "HΦ".
-      iDestruct "HRes" as "[[-> HInh]|(-> & HPerm & HR)]".
-      all: wp_pures.
-      - iApply "HΦ".
-        iLeft; by iFrame.
-      - iAssert (▷ thread_has_permit γth)%I with "[$]" as "HHasPerm".
-        iClear "HIntHandle HSemInv HPermInv HSegLoc HRend". clear.
-        awp_apply (thread_update_state _ _ _ true with "HThreadHandle") without "HΦ HR".
-        iAaccIntro with "HHasPerm".
-        by iIntros "$ //".
-        iIntros "HNoPerms !> [HΦ HR]".
-        wp_pures. iApply "HΦ".
-        iRight; iFrame. by iExists _.
-    }
-    {
-      iIntros (Φ') "!> [HInhTok #HInterrupted] HΦ'". wp_pures. wp_bind (FAA _ _).
-      move: namespaces_disjoint. clear. intros.
-      iInv "HSemInv" as (availablePermits v)
-                          "(HPerms & >HAuth & HTq & Hp & >HPure)" "HInvClose".
-
-      remember (availablePermits - _)%Z as oldP.
-      destruct (decide (0 <= oldP)%Z) as [HLt|HGt].
-      {
-        wp_faa.
-        iInv "HPermInv" as (?) ">HFrag" "HPermsClose".
-        iDestruct (own_valid_2 with "HAuth HFrag") as
-              %[->%Excl_included%leibniz_equiv _]%auth_both_valid.
-        iMod (own_update_2 with "HAuth HFrag") as "[HAuth HFrag]".
-        {
-          apply auth_update, option_local_update.
-          apply (exclusive_local_update _ (Excl (availablePermits + 1)%nat)).
-          done.
-        }
-        iMod ("HPermsClose" with "[HFrag]") as "_"; first by eauto.
-        iAssert (⌜v = 0%nat⌝)%I as %->.
-        by iDestruct "HPure" as %[HH|HH]; subst; iPureIntro; lia.
-        subst. rewrite Z.sub_0_r.
-        iMod (thread_queue_abandon_if_empty with "HInhTok HTq")
-          as "(HTq & HR & #HDone)".
-        iMod ("HInvClose" with "[-HΦ']") as "_".
-        {
-          iExists _, _. iFrame. rewrite seq_add big_sepL_app /=. iFrame.
-          iSplitL; last by iPureIntro; eauto.
-          by rewrite Z.sub_0_r Nat2Z.inj_add.
-        }
-        iModIntro. wp_pures. rewrite bool_decide_decide decide_True //; last lia.
-        wp_pures.
-        iApply "HΦ'".
-        iLeft. by iFrame "HInterrupted".
-      }
-
-      iMod (do_cancel_rendezvous_as_counter_spec with "HInhTok HTq")
-        as "[HTq HTT]"; first by lia.
-
-      wp_faa.
-
-      iDestruct "HTT" as "[(HCancTok & #HRendCanc) | (HLoc & HAwak & #HRendRes)]".
-      2: {
-        iMod ("HInvClose" with "[-HΦ' HAwak HLoc]") as "_".
-        {
-          iExists _, _. iFrame.
-          iSplitR "HPure"; last by iDestruct "HPure" as "[->|%]"; iPureIntro; lia.
-          subst.
-          by replace (availablePermits - v + 1)%Z
-            with (availablePermits - (v - 1)%nat)%Z by lia.
-        }
-        iModIntro. wp_pures. rewrite bool_decide_decide decide_False //.
-        wp_pures. wp_lam. wp_lam. wp_pures.
-
-        awp_apply (segment_data_at_spec) without "HΦ' HLoc HAwak".
-        by iPureIntro; apply Nat.mod_upper_bound; lia.
-        iInv "HSemInv" as (? ?) "(HHead1 & HHead2 & HTq & HTail)".
-        iDestruct "HTq" as (? ?) "[(HInfArr & HTail') HTail'']".
-        iDestruct (is_segment_by_location with "HSegLoc HInfArr")
-          as (? ?) "[HIsSeg HInfArrRestore]".
-        iAaccIntro with "HIsSeg".
-        {
-          iIntros "HIsSeg".
-          iDestruct ("HInfArrRestore" with "HIsSeg") as "HInfArr".
-          iIntros "!>". iSplitL; last done.
-          iExists _, _. iFrame. iExists _, _. iFrame.
-        }
-
-        iIntros (?) "(HIsSeg & #HArrMapsto & #HCellInv)".
-        iDestruct (bi.later_wand with "HInfArrRestore HIsSeg") as "HInfArr".
-        iSplitL; first by iExists _, _; iFrame; iExists _, _; iFrame.
-        iIntros "!> (HΦ' & HLoc & HAwak)". wp_pures.
-
-        iDestruct "HLoc" as (ℓ) "[#HArrMapsto' Hℓ]".
-        iDestruct (array_mapsto'_agree with "HArrMapsto HArrMapsto'") as %->.
-        iAssert (▷ ℓ ↦ RESUMEDV)%I with "Hℓ" as "Hℓ".
-        awp_apply getAndSet.getAndSet_spec without "HΦ' HAwak".
-        iAssert (▷ ℓ ↦ RESUMEDV ∧ ⌜val_is_unboxed RESUMEDV⌝)%I
-          with "[Hℓ]" as "HAacc".
-        by iFrame.
-        iAaccIntro with "HAacc".
-        by iIntros "[$ _]".
-        iIntros "Hℓ !> [HΦ' HAwak]".
-        wp_pures.
-        wp_apply (resume_in_semaphore_spec with "[$] [$] [$]").
-        iIntros "_". wp_pures. iApply "HΦ'". iLeft. by iFrame "HInterrupted".
-      }
-
-      iMod ("HInvClose" with "[-HΦ' HCancTok]") as "_".
-      {
-        iExists _, _. iFrame.
-        iSplitL "Hp"; last by iDestruct "HPure" as "[->|%]"; by (iPureIntro; lia).
-        subst.
-        by replace (availablePermits - v + 1)%Z with
-            (availablePermits - (v - 1)%nat)%Z by lia.
-      }
-
-      iModIntro. wp_pures. rewrite bool_decide_decide decide_False //. wp_pures.
-      awp_apply (cancel_cell_spec with "HRendCanc HSegLoc HCancTok") without "HΦ'".
-      iInv "HSemInv" as (? ?) "(HHead1 & HHead2 & HTq & HTail)".
-      iDestruct "HTq" as (? ?) "[HTq HTail'']".
-      iAaccIntro with "HTq".
-      {
-        iIntros "HTq !>". iSplitL; last done. iExists _, _. iFrame.
-        iExists _, _. iFrame.
-      }
-      iIntros (b) "[HTq HRes] !>".
-      iSplitR "HRes".
-      { iExists _, _. iFrame. iExists _, _. iFrame. }
-      iIntros "HΦ'".
-      iDestruct "HRes" as "[(-> & HAwak)|->]"; wp_pures.
-      wp_apply (resume_in_semaphore_spec with "[$] [$] [$]").
-      iIntros "_"; wp_pures.
-      all: iApply "HΦ'"; iLeft; by iFrame "HInterrupted".
-    }
-  }
-  iIntros (? ?) "[(-> & [-> #HInterrupted])|(-> & -> & HHasPerm & HR)]".
-  1: by wp_pures; iApply "HΦ"; iRight; eauto.
-  iApply "HΦ". iLeft. iFrame. done.
+Theorem cancelSemaphoreFuture_spec R γa γtq γe γd s γf f:
+  is_semaphore R γa γtq γe γd s -∗
+  is_semaphore_future R γtq γa γf f -∗
+  <<< ▷ thread_queue_future_cancellation_permit γf >>>
+    cancelSemaphoreFuture array_interface s f @ ⊤ ∖ ↑NFuture ∖ ↑N
+  <<< ∃ (r: bool),
+      if r then future_is_cancelled γf
+      else (∃ v, ▷ future_is_completed γf v) ∗
+           thread_queue_future_cancellation_permit γf, RET #r >>>.
+Proof.
+  iIntros "#HIsSem #HFuture" (Φ) "AU".
+  iDestruct "HIsSem" as (e d p ->) "[HInv HTq]". wp_lam. wp_pures. wp_lam.
+  wp_pures. awp_apply (try_cancel_thread_queue_future with "HTq HFuture");
+              first by solve_ndisj.
+  iApply (aacc_aupd_commit with "AU"). by solve_ndisj.
+  iIntros "HCancPermit". iAaccIntro with "HCancPermit". by iIntros "$ !> $ !>".
+  iIntros (r) "Hr". iExists r. destruct r.
+  2: { iDestruct "Hr" as "[$ $]". iIntros "!> HΦ !>". by wp_pures. }
+  iDestruct "Hr" as "[#HFutureCancelled Hr]". iFrame "HFutureCancelled".
+  rewrite /is_semaphore_future /is_thread_queue_future.
+  iDestruct "Hr" as (i f' s ->) "Hr"=> /=.
+  iDestruct "Hr" as "(#H↦~ & #HTh & HToken)". iIntros "!> HΦ !>". wp_pures.
+  wp_lam. wp_pures. wp_apply derefCellPointer_spec.
+  by iDestruct "HTq" as "(_ & $ & _)". iIntros (ℓ) "#H↦". wp_pures.
+  wp_bind (FAA _ _).
+  iInv "HInv" as (availablePermits) "[HRs HOpen]" "HClose".
+  iDestruct "HOpen" as (enqueuedThreads) "(>HState & Hp & >HPures)".
+  iDestruct "HPures" as %HPures.
+  iMod (register_cancellation with "HTq HToken HState")
+       as "[HCancToken HState]"; first by solve_ndisj.
+  destruct (decide (availablePermits - enqueuedThreads < 0)%Z) as [HLt|HGe].
+  - assert (availablePermits = 0) as -> by lia.
+    destruct enqueuedThreads as [|enqueuedThreads']=>/=; first lia.
+    iDestruct "HState" as "(HState & HCancHandle & #HInhabited)".
+    wp_faa.
+    iMod ("HClose" with "[-HΦ HCancToken HCancHandle]") as "_".
+    { iExists 0. iSplitR; simpl; first done. iExists enqueuedThreads'.
+      rewrite Nat.sub_0_r. iFrame "HState". iSplitL; last by iLeft.
+      by replace (0%nat - S enqueuedThreads' + 1)%Z
+        with (0%nat - enqueuedThreads')%Z by lia. }
+    iModIntro. wp_pures. wp_bind (getAndSet.getAndSet _ _).
+    awp_apply (markCancelled_spec with "HTq HInhabited H↦ HCancToken HTh")
+              without "HΦ HCancHandle".
+    iAaccIntro with "[//]"; first done. iIntros (v) "Hv"=>/=.
+    iIntros "!> [HΦ HCancHandle]". wp_pures.
+    iAssert (▷ cell_cancellation_handle _ _ _ _ _ _)%I
+            with "[HCancHandle]" as "HCancHandle"; first done.
+    awp_apply (cancelCell_spec with "[] H↦~") without "Hv HΦ".
+    by iDestruct "HTq" as "(_ & $ & _)".
+    iAaccIntro with "HCancHandle". by iIntros "$".
+    iIntros "#HCancelled !> [Hv HΦ]". wp_pures.
+    iDestruct "Hv" as "[[-> _]|Hv]"; first by wp_pures.
+    iDestruct "Hv" as (x ->) "(#HInhabited' & HAwak & %)"; simplify_eq.
+    wp_pures. wp_apply (resumeSemaphore_spec with "[$]").
+    iIntros (r) "Hr". destruct r; wp_pures; first done.
+    wp_apply (releaseSemaphore_spec with "[Hr]").
+    { iSplitR; last by iApply "Hr". iExists _, _, _.
+      iSplitR; first done. iFrame "HInv HTq". }
+    iIntros "_". by wp_pures.
+  - rewrite bool_decide_true; last lia. assert (enqueuedThreads = 0) as -> by lia.
+    simpl. iDestruct "HState" as "(HState & HR & #HInhabited)".
+    wp_faa.
+    iMod ("HClose" with "[-HΦ HCancToken]") as "_".
+    { iExists (S availablePermits). iFrame "HR HRs". iExists 0.
+      iFrame "HState". iSplitL; last by iRight.
+      by replace (availablePermits - 0%nat + 1)%Z
+        with (S availablePermits - 0%nat)%Z by lia. }
+    iModIntro. wp_pures. rewrite bool_decide_false; last lia. wp_pures.
+    wp_bind (getAndSet.getAndSet _ _).
+    awp_apply (markRefused_spec with "HTq HInhabited H↦ HCancToken HTh [//]")
+              without "HΦ".
+    iAaccIntro with "[//]"; first done. iIntros (v) "Hv"=>/=.
+    iIntros "!> HΦ". iDestruct "Hv" as "[[-> _]|Hv]"; first by wp_pures.
+    iDestruct "Hv" as (? ->) "[_ >%]". simplify_eq. by wp_pures.
 Qed.
 
 End proof.
