formal-proofs/theories/lib/concurrent_linked_list/infinite_array/array_spec.v
@@ -51,9 +51,9 @@ Record infiniteArraySpec Σ `{!heapG Σ} (impl: infiniteArrayInterface) :=
       cancelCell_spec N γ co p i:
         is_infinite_array N γ co -∗
         is_infinite_array_cell_pointer N γ p i -∗
-        <<< cell_cancellation_handle N γ i >>>
+        <<< ▷ cell_cancellation_handle N γ i >>>
             cancelCell impl p @ ⊤ ∖ ↑N
-        <<< cell_is_cancelled N γ i, RET #() >>>;
+        <<< ▷ cell_is_cancelled N γ i, RET #() >>>;
       findCell_spec N γ co p (source_id id: nat):
         {{{ is_infinite_array N γ co ∗
             is_infinite_array_cutoff_reading N γ p source_id }}}
